<?xml version="1.0"?>
<rdf:RDF xmlns="http://data.europa.eu/esco/flow#"
     xml:base="http://data.europa.eu/esco/flow"
     xmlns:rdfs="http://www.w3.org/2000/01/rdf-schema#"
     xmlns:owl2xml="http://www.w3.org/2006/12/owl2-xml#"
     xmlns:owl="http://www.w3.org/2002/07/owl#"
     xmlns:xsd="http://www.w3.org/2001/XMLSchema#"
     xmlns:rdf="http://www.w3.org/1999/02/22-rdf-syntax-ns#"
     xmlns:skos-xl="http://www.w3.org/2008/05/skos-xl#"
     xmlns:skos="http://www.w3.org/2004/02/skos/core#">
    <owl:Ontology rdf:about="http://data.europa.eu/esco/flow">
        <owl:versionInfo rdf:datatype="http://www.w3.org/2001/XMLSchema#string">1.0</owl:versionInfo>
        <owl:imports rdf:resource="http://www.w3.org/2004/02/skos/core"/>
        <owl:imports rdf:resource="http://www.w3.org/2008/05/skos-xl"/>
    </owl:Ontology>
    


    <!-- 
    ///////////////////////////////////////////////////////////////////////////////////////
    //
    // Object Properties
    //
    ///////////////////////////////////////////////////////////////////////////////////////
     -->

    


    <!-- http://data.europa.eu/esco/flow#exportedThesaurus -->

    <owl:ObjectProperty rdf:about="http://data.europa.eu/esco/flow#exportedThesaurus">
        <rdfs:label xml:lang="en">published theasurus</rdfs:label>
        <rdfs:comment xml:lang="en">The referenced subject provides the publishing details of the thesaurus denoted by the object value.</rdfs:comment>
        <rdfs:isDefinedBy rdf:resource="http://data.europa.eu/esco/flow"/>
        <rdfs:domain rdf:resource="http://data.europa.eu/esco/flow#Export"/>
        <rdfs:range rdf:resource="http://www.w3.org/2004/02/skos/core#ConceptScheme"/>
    </owl:ObjectProperty>
    


    <!-- 
    ///////////////////////////////////////////////////////////////////////////////////////
    //
    // Data properties
    //
    ///////////////////////////////////////////////////////////////////////////////////////
     -->

    


    <!-- http://data.europa.eu/esco/flow#approvedForRelease -->

    <owl:DatatypeProperty rdf:about="http://data.europa.eu/esco/flow#approvedForRelease">
        <rdfs:label xml:lang="en">approved for release</rdfs:label>
        <rdfs:seeAlso rdf:datatype="http://www.w3.org/2001/XMLSchema#anyURI">http://data.europa.eu/esco/flow#exportVersion</rdfs:seeAlso>
        <rdfs:seeAlso rdf:datatype="http://www.w3.org/2001/XMLSchema#anyURI">http://data.europa.eu/esco/flow#status</rdfs:seeAlso>
        <rdfs:comment xml:lang="en">The value provides the expected  release number for the official release of a new or modified  concept.
The property will only be present in intermediate maintenance releases.
In general, a maintenance release is not published.</rdfs:comment>
        <rdfs:isDefinedBy rdf:resource="http://data.europa.eu/esco/flow"/>
        <rdfs:range rdf:resource="http://www.w3.org/2001/XMLSchema#string"/>
        <rdfs:domain>
            <owl:Class>
                <owl:unionOf rdf:parseType="Collection">
                    <rdf:Description rdf:about="http://www.w3.org/2004/02/skos/core#Concept"/>
                    <rdf:Description rdf:about="http://www.w3.org/2004/02/skos/core#ConceptScheme"/>
                    <rdf:Description rdf:about="http://www.w3.org/2004/02/skos/core#Collection"/>
                    <rdf:Description rdf:about="http://www.w3.org/2008/05/skos-xl#Label"/>
                </owl:unionOf>
            </owl:Class>
        </rdfs:domain>
    </owl:DatatypeProperty>
    


    <!-- http://data.europa.eu/esco/flow#editable -->

    <owl:DatatypeProperty rdf:about="http://data.europa.eu/esco/flow#editable">
        <rdfs:label xml:lang="en">editable</rdfs:label>
        <rdfs:comment rdf:datatype="http://www.w3.org/2001/XMLSchema#string">indicates if Concepts belonging to the Concept Scheme are editable or read-only (used or inherited) in the ESCO context.
The default value is &apos;true&apos;. 
However, in the case of &apos;false&apos; skos-xl:Label(s) still can be changed to be more adapted to the ESCO audience.</rdfs:comment>
        <rdfs:isDefinedBy rdf:resource="http://data.europa.eu/esco/flow"/>
        <rdfs:range rdf:resource="http://www.w3.org/2001/XMLSchema#boolean"/>
        <rdfs:domain rdf:resource="http://www.w3.org/2004/02/skos/core#ConceptScheme"/>
    </owl:DatatypeProperty>
    


    <!-- http://data.europa.eu/esco/flow#exportDate -->

    <owl:DatatypeProperty rdf:about="http://data.europa.eu/esco/flow#exportDate">
        <rdf:type rdf:resource="http://www.w3.org/2002/07/owl#FunctionalProperty"/>
        <rdfs:label xml:lang="en">export date</rdfs:label>
        <rdfs:comment xml:lang="en">The system date and time at which the described  thesaurus release is published.</rdfs:comment>
        <rdfs:isDefinedBy rdf:resource="http://data.europa.eu/esco/flow"/>
        <rdfs:domain rdf:resource="http://data.europa.eu/esco/flow#Export"/>
        <rdfs:range rdf:resource="http://www.w3.org/2001/XMLSchema#dateTime"/>
    </owl:DatatypeProperty>
    


    <!-- http://data.europa.eu/esco/flow#exportVersion -->

    <owl:DatatypeProperty rdf:about="http://data.europa.eu/esco/flow#exportVersion">
        <rdf:type rdf:resource="http://www.w3.org/2002/07/owl#FunctionalProperty"/>
        <rdfs:label xml:lang="en">exported thesaurus release number</rdfs:label>
        <rdfs:comment xml:lang="en">The release number is the version identier of the published thesaurus.</rdfs:comment>
        <rdfs:isDefinedBy rdf:resource="http://data.europa.eu/esco/flow"/>
        <rdfs:domain rdf:resource="http://data.europa.eu/esco/flow#Export"/>
        <rdfs:range rdf:resource="http://www.w3.org/2001/XMLSchema#string"/>
    </owl:DatatypeProperty>
    


    <!-- http://data.europa.eu/esco/flow#identifier -->

    <owl:DatatypeProperty rdf:about="http://data.europa.eu/esco/flow#identifier">
        <rdf:type rdf:resource="http://www.w3.org/2002/07/owl#FunctionalProperty"/>
        <rdfs:label xml:lang="en">ITM identifier</rdfs:label>
        <rdfs:comment xml:lang="en">ITM identifier is generated by a sequence, portable from an ITM installation to another, whereas topic id is linked to a specific ITM data base.</rdfs:comment>
        <rdfs:isDefinedBy rdf:resource="http://data.europa.eu/esco/flow"/>
        <rdfs:range rdf:resource="http://www.w3.org/2001/XMLSchema#string"/>
    </owl:DatatypeProperty>
    

    <!-- http://data.europa.eu/esco/flow#intermediateRelease -->

    <owl:DatatypeProperty rdf:about="http://data.europa.eu/esco/flow#intermediateRelease">
        <rdfs:label xml:lang="en">intermediate release</rdfs:label>
        <rdfs:comment xml:lang="en">true: Indicates this is a realease including the terms and concepts that were approved in the ESCO back-office maintenace workspace.
Not present or false indicate this is a release of the publishing ESCO back-office workspace.</rdfs:comment>
        <rdfs:isDefinedBy rdf:resource="http://data.europa.eu/esco/flow"/>
        <rdfs:domain rdf:resource="http://data.europa.eu/esco/flow#Export"/>
        <rdfs:range rdf:resource="http://www.w3.org/2001/XMLSchema#boolean"/>
    </owl:DatatypeProperty>
    


    <!-- http://data.europa.eu/esco/flow#releasedWithVersion -->

    <owl:DatatypeProperty rdf:about="http://data.europa.eu/esco/flow#releasedWithVersion">
        <rdfs:label xml:lang="en">released with version</rdfs:label>
        <rdfs:seeAlso rdf:datatype="http://www.w3.org/2001/XMLSchema#anyURI">http://data.europa.eu/esco/flow#exportVersion</rdfs:seeAlso>
        <rdfs:comment xml:lang="en">The release number in which the term was added.
The fixed string &apos;n/a&apos; indicates the historic release number is not available.</rdfs:comment>
        <rdfs:isDefinedBy rdf:resource="http://data.europa.eu/esco/flow"/>
        <rdfs:range rdf:resource="http://www.w3.org/2001/XMLSchema#string"/>
        <rdfs:domain>
            <owl:Class>
                <owl:unionOf rdf:parseType="Collection">
                    <rdf:Description rdf:about="http://www.w3.org/2004/02/skos/core#Concept"/>
                    <rdf:Description rdf:about="http://www.w3.org/2004/02/skos/core#ConceptScheme"/>
                    <rdf:Description rdf:about="http://www.w3.org/2004/02/skos/core#Collection"/>
                    <rdf:Description rdf:about="http://www.w3.org/2008/05/skos-xl#Label"/>
                </owl:unionOf>
            </owl:Class>
        </rdfs:domain>
    </owl:DatatypeProperty>
    


    <!-- http://data.europa.eu/esco/flow#status -->

    <owl:DatatypeProperty rdf:about="http://data.europa.eu/esco/flow#status">
        <rdfs:label rdf:datatype="http://www.w3.org/2001/XMLSchema#string">status</rdfs:label>
        <rdfs:comment xml:lang="en">The position or state of the concept or label (term) with respect to the back-office maintenance workflow.
Three states are relevant for a publication:
- &apos;valid&apos;: for released terms and concepts
- &apos;to be translated&apos;: A term requiring further translation
  look at ev:toBeTranslated to find the outstanding translations
- &apos;in maintenance&apos;: a concept or term in maintenance.
  look at ev:approvedForRelease to know for which version the approval holds.

If the property is not present, &apos;valid&apos; must be assumed.

The property is typically set on a maintenance release only.</rdfs:comment>
        <rdfs:isDefinedBy rdf:resource="http://data.europa.eu/esco/flow"/>
        <rdfs:domain>
            <owl:Class>
                <owl:unionOf rdf:parseType="Collection">
                    <rdf:Description rdf:about="http://www.w3.org/2004/02/skos/core#Concept"/>
                    <rdf:Description rdf:about="http://www.w3.org/2008/05/skos-xl#Label"/>
                </owl:unionOf>
            </owl:Class>
        </rdfs:domain>
        <rdfs:range>
            <rdfs:Datatype>
                <owl:oneOf>
                    <rdf:Description>
                        <rdf:type rdf:resource="http://www.w3.org/1999/02/22-rdf-syntax-ns#List"/>
                        <rdf:first rdf:datatype="http://www.w3.org/2001/XMLSchema#string">in maintenance</rdf:first>
                        <rdf:rest>
                            <rdf:Description>
                                <rdf:type rdf:resource="http://www.w3.org/1999/02/22-rdf-syntax-ns#List"/>
                                <rdf:first rdf:datatype="http://www.w3.org/2001/XMLSchema#string">to be translated</rdf:first>
                                <rdf:rest>
                                    <rdf:Description>
                                        <rdf:type rdf:resource="http://www.w3.org/1999/02/22-rdf-syntax-ns#List"/>
                                        <rdf:first rdf:datatype="http://www.w3.org/2001/XMLSchema#string">valid</rdf:first>
                                        <rdf:rest rdf:resource="http://www.w3.org/1999/02/22-rdf-syntax-ns#nil"/>
                                    </rdf:Description>
                                </rdf:rest>
                            </rdf:Description>
                        </rdf:rest>
                    </rdf:Description>
                </owl:oneOf>
            </rdfs:Datatype>
        </rdfs:range>
    </owl:DatatypeProperty>
    


    <!-- http://data.europa.eu/esco/flow#toBeTranslated -->

    <owl:DatatypeProperty rdf:about="http://data.europa.eu/esco/flow#toBeTranslated">
        <rdfs:label rdf:datatype="http://www.w3.org/2001/XMLSchema#string">to be translated</rdfs:label>
        <rdfs:comment xml:lang="en">The range value must have
- language (the language for which translatioin is required)
- for a term this must be the language of the term
- for a microthesaurus or domain this may be a comma seperated list of languages.

The format is:
&lt;lang&gt; [ ,&apos;&lt;lang&gt; ]*</rdfs:comment>
        <rdfs:isDefinedBy rdf:resource="http://data.europa.eu/esco/flow"/>
        <rdfs:domain>
            <owl:Class>
                <owl:unionOf rdf:parseType="Collection">
                    <rdf:Description rdf:about="http://www.w3.org/2004/02/skos/core#ConceptScheme"/>
                    <rdf:Description rdf:about="http://www.w3.org/2008/05/skos-xl#Label"/>
                </owl:unionOf>
            </owl:Class>
        </rdfs:domain>
    </owl:DatatypeProperty>
    


    <!-- 
    ///////////////////////////////////////////////////////////////////////////////////////
    //
    // Classes
    //
    ///////////////////////////////////////////////////////////////////////////////////////
     -->

    


    <!-- http://data.europa.eu/esco/flow#Export -->

    <owl:Class rdf:about="http://data.europa.eu/esco/flow#Export">
        <rdfs:label xml:lang="en">current thesaurus export</rdfs:label>
        <rdfs:subClassOf rdf:resource="http://www.w3.org/2002/07/owl#Thing"/>
        <rdfs:subClassOf>
            <owl:Restriction>
                <owl:onProperty rdf:resource="http://data.europa.eu/esco/flow#exportedThesaurus"/>
                <owl:cardinality rdf:datatype="http://www.w3.org/2001/XMLSchema#nonNegativeInteger">1</owl:cardinality>
            </owl:Restriction>
        </rdfs:subClassOf>
        <rdfs:subClassOf>
            <owl:Restriction>
                <owl:onProperty rdf:resource="http://data.europa.eu/esco/flow#exportDate"/>
                <owl:qualifiedCardinality rdf:datatype="http://www.w3.org/2001/XMLSchema#nonNegativeInteger">1</owl:qualifiedCardinality>
                <owl:onDataRange rdf:resource="http://www.w3.org/2001/XMLSchema#dateTime"/>
            </owl:Restriction>
        </rdfs:subClassOf>
        <rdfs:subClassOf>
            <owl:Restriction>
                <owl:onProperty rdf:resource="http://data.europa.eu/esco/flow#exportVersion"/>
                <owl:qualifiedCardinality rdf:datatype="http://www.w3.org/2001/XMLSchema#nonNegativeInteger">1</owl:qualifiedCardinality>
                <owl:onDataRange rdf:resource="http://www.w3.org/2001/XMLSchema#string"/>
            </owl:Restriction>
        </rdfs:subClassOf>
        <rdfs:isDefinedBy rdf:datatype="http://www.w3.org/2001/XMLSchema#anyURI">http://data.europa.eu/esco/flow</rdfs:isDefinedBy>
        <rdfs:comment xml:lang="en">A utility class capturing the publication characteristics of the exported ESCO thesaurus release.

The export details are provided by a back-office export from the ESCO thesaurus management system.</rdfs:comment>
    </owl:Class>
    


    <!-- http://www.w3.org/2002/07/owl#Thing -->

    <owl:Class rdf:about="http://www.w3.org/2002/07/owl#Thing"/>
    


    <!-- http://www.w3.org/2004/02/skos/core#Concept -->

    <owl:Class rdf:about="http://www.w3.org/2004/02/skos/core#Concept"/>
    


    <!-- http://www.w3.org/2004/02/skos/core#ConceptScheme -->

    <owl:Class rdf:about="http://www.w3.org/2004/02/skos/core#ConceptScheme"/>
    


    <!-- http://www.w3.org/2008/05/skos-xl#Label -->

    <owl:Class rdf:about="http://www.w3.org/2008/05/skos-xl#Label"/>
</rdf:RDF>



<!-- Generated by the OWL API (version 3.4.2) http://owlapi.sourceforge.net -->

